WIP CBOR.Spec.Raw.Sort

src/cbor/spec/raw/CBOR.Spec.Raw.Sort.fsti
@@ -50,64 +50,9 @@ let cbor_raw_sort_elem
   | Map len v -> Map len (cbor_map_sort_failsafe v)
   | _ -> x
 
-let cbor_raw_sort_elem_ints_optimal
-  (x: raw_data_item)
-: Lemma
-  (requires (raw_data_item_ints_optimal x == true))
-  (ensures (raw_data_item_ints_optimal (cbor_raw_sort_elem x) == true))
-= assert_norm (raw_data_item_ints_optimal == holds_on_raw_data_item raw_data_item_ints_optimal_elem);
-  holds_on_raw_data_item_eq raw_data_item_ints_optimal_elem x;
-  holds_on_raw_data_item_eq raw_data_item_ints_optimal_elem (cbor_raw_sort_elem x);
-  match x with
-  | Map len v ->
-    list_for_all_intro (holds_on_pair raw_data_item_ints_optimal) (cbor_map_sort_failsafe v) (fun x ->
-      List.Tot.for_all_mem (holds_on_pair raw_data_item_ints_optimal) v
-    )
-  | _ -> ()
-
-let cbor_raw_sort_elem_equiv
-  (x: raw_data_item)
-: Lemma
-  (ensures (raw_equiv x (cbor_raw_sort_elem x) == true))
-= admit ()
-(*
-  raw_equiv_eq x (cbor_raw_sort_elem x);
-  match x with
-  | Map len v ->
-    list_for_all_intro (list_existsb2 (holds_on_pair2 raw_equiv) (cbor_map_sort_failsafe v)) v (fun x ->
-      raw_equiv_refl (fst x);
-      raw_equiv_refl (snd x);
-      list_existsb_intro (holds_on_pair2 raw_equiv x) (cbor_map_sort_failsafe v) x
-    );
-    list_for_all_intro (list_existsb2 (holds_on_pair2 raw_equiv) v) (cbor_map_sort_failsafe v) (fun x ->
-      raw_equiv_refl (fst x);
-      raw_equiv_refl (snd x);
-      list_existsb_intro (holds_on_pair2 raw_equiv x) v x
-    )
-  | _ -> raw_equiv_refl x
-*)
-
 let cbor_raw_sort = raw_data_item_fmap cbor_raw_sort_elem
 
-let cbor_raw_sort_ints_optimal
-  (x: raw_data_item)
-: Lemma
-  (requires (raw_data_item_ints_optimal x == true))
-  (ensures (raw_data_item_ints_optimal (cbor_raw_sort x) == true))
-= holds_on_raw_data_item_fmap_inv
-    cbor_raw_sort_elem
-    raw_data_item_ints_optimal_elem
-    (fun x -> holds_on_raw_data_item_eq raw_data_item_ints_optimal_elem x)
-    (fun x -> cbor_raw_sort_elem_ints_optimal x)
-    x
-
-let cbor_raw_sort_equiv
-  (x: raw_data_item)
-: Lemma
-  (ensures (raw_equiv x (cbor_raw_sort x) == true))
-= admit () // raw_equiv_fmap cbor_raw_sort_elem cbor_raw_sort_elem_equiv x
-
-let cbor_raw_sort_correct
+val cbor_raw_sort_correct
   (x: raw_data_item)
 : Lemma
   (requires (raw_data_item_ints_optimal x == true /\
@@ -117,51 +62,8 @@ let cbor_raw_sort_correct
     let x' = cbor_raw_sort x in
     raw_data_item_ints_optimal x' == true /\
     raw_data_item_sorted deterministically_encoded_cbor_map_key_order x' == true /\
-    valid_raw_data_item x'  == true
+    valid_raw_data_item x'  == true /\
+    raw_equiv x x'
   ))
-= admit ()
-(*
-holds_on_raw_data_item_andp raw_data_item_ints_optimal_elem (valid_item basic_data_model) x;
-  valid_eq' basic_data_model x;
-  valid_eq' basic_data_model (cbor_raw_sort x);
-  let phi = andp raw_data_item_ints_optimal_elem
-    (valid_item basic_data_model) in
-  let so = raw_data_item_sorted_elem deterministically_encoded_cbor_map_key_order in
-  holds_on_raw_data_item_fmap_gen
-    cbor_raw_sort_elem
-    phi
-    so
-    (fun x ->
-      let x' = pre_raw_data_item_fmap cbor_raw_sort_elem x in
-      holds_on_raw_data_item_eq phi x;
-      pre_holds_on_raw_data_item_implies (phi `andp` so) phi (fun _ -> ()) x';
-      match x with
-      | Map _ v ->
-        valid_raw_data_item_map_fmap_equiv
-          basic_data_model
-          (raw_data_item_fmap cbor_raw_sort_elem)
-          v
-          (fun x -> cbor_raw_sort_equiv x)
-      | _ -> ()
-    )
-    (fun x ->
-      holds_on_raw_data_item_andp raw_data_item_ints_optimal_elem (valid_item basic_data_model) x;
-      let x' = cbor_raw_sort_elem x in
-      holds_on_raw_data_item_andp phi so x';
-      holds_on_raw_data_item_andp raw_data_item_ints_optimal_elem (valid_item basic_data_model) x';
-      cbor_raw_sort_elem_ints_optimal x;
-      match x with
-      | Map len v ->
-        valid_raw_data_item_map_no_repeats v;
-        cbor_map_sort_failsafe_correct v;
-        list_for_all_intro (holds_on_pair (holds_on_raw_data_item so)) (cbor_map_sort_failsafe v) (fun _ ->
-          List.Tot.for_all_mem (holds_on_pair (holds_on_raw_data_item so)) v
-        );
-        raw_data_item_sorted_optimal_valid deterministically_encoded_cbor_map_key_order x'
-      | _ -> ()
-    )
-    x;
-  let x' = cbor_raw_sort x in
-  holds_on_raw_data_item_andp phi (raw_data_item_sorted_elem deterministically_encoded_cbor_map_key_order) x';
-  holds_on_raw_data_item_andp raw_data_item_ints_optimal_elem (valid_item basic_data_model) x'
-*)
+
+let cbor_raw_sort_equiv = cbor_raw_sort_correct
