src/cbor/spec/raw/CBOR.Spec.API.Format.fst
@@ -43,9 +43,11 @@ let cbor_det_serialize_tag_length tag =
   RF.serialize_cbor_tag_length (RV.mk_raw_uint64 tag)
 
 let cbor_det_serialize_tag_correct tag payload =
-  R.mk_cbor_eq (R.Tagged (RV.mk_raw_uint64 tag) (R.mk_det_raw_cbor payload));
-  R.mk_det_raw_cbor_mk_cbor (R.Tagged (RV.mk_raw_uint64 tag) (R.mk_det_raw_cbor payload));
-  assert (R.mk_det_raw_cbor (pack (CTagged tag payload)) == R.Tagged (RV.mk_raw_uint64 tag) (R.mk_det_raw_cbor payload));
+  let x = (R.Tagged (RV.mk_raw_uint64 tag) (R.mk_det_raw_cbor payload)) in
+  R.valid_eq R.basic_data_model x;
+  R.mk_cbor_eq x;
+  R.mk_det_raw_cbor_mk_cbor x;
+  assert (R.mk_det_raw_cbor (pack (CTagged tag payload)) == x);
   RF.serialize_cbor_tag_correct (RV.mk_raw_uint64 tag) (R.mk_det_raw_cbor payload)
 
 let rec list_map_mk_det_raw_cbor_correct
@@ -97,6 +99,7 @@ let cbor_det_serialize_string_length_gt ty l =
   let len = R.mk_raw_uint64 (U64.uint_to_t (Seq.length l)) in
   assert (RV.raw_uint64_optimal len);
   let x = R.String ty len l in
+  R.valid_eq R.basic_data_model x;
   R.mk_cbor_eq x;
   R.mk_det_raw_cbor_mk_cbor x;
   RF.serialize_cbor_string_length_gt ty len l;
